src/HOL/Lambda/Type.thy
@@ -45,8 +45,18 @@ datatype type =
     Atom nat
   | Fun type type    (infixr "\<Rightarrow>" 200)
 
+inductive2 typing :: "(nat \<Rightarrow> type) \<Rightarrow> dB \<Rightarrow> type \<Rightarrow> bool"  ("_ \<turnstile> _ : _" [50, 50, 50] 50)
+  where
+    Var [intro!]: "env x = T \<Longrightarrow> env \<turnstile> Var x : T"
+  | Abs [intro!]: "env\<langle>0:T\<rangle> \<turnstile> t : U \<Longrightarrow> env \<turnstile> Abs t : (T \<Rightarrow> U)"
+  | App [intro!]: "env \<turnstile> s : T \<Rightarrow> U \<Longrightarrow> env \<turnstile> t : T \<Longrightarrow> env \<turnstile> (s \<degree> t) : U"
+
+inductive_cases2 typing_elims [elim!]:
+  "e \<turnstile> Var i : T"
+  "e \<turnstile> t \<degree> u : T"
+  "e \<turnstile> Abs t : T"
+
 consts
-  typing :: "((nat \<Rightarrow> type) \<times> dB \<times> type) set"
   typings :: "(nat \<Rightarrow> type) \<Rightarrow> dB list \<Rightarrow> type list \<Rightarrow> bool"
 
 abbreviation
@@ -54,31 +64,13 @@ abbreviation
   "Ts =>> T == foldr Fun Ts T"
 
 abbreviation
-  typing_rel :: "(nat \<Rightarrow> type) \<Rightarrow> dB \<Rightarrow> type \<Rightarrow> bool"  ("_ |- _ : _" [50, 50, 50] 50) where
-  "env |- t : T == (env, t, T) \<in> typing"
-
-abbreviation
   typings_rel :: "(nat \<Rightarrow> type) \<Rightarrow> dB list \<Rightarrow> type list \<Rightarrow> bool"
     ("_ ||- _ : _" [50, 50, 50] 50) where
   "env ||- ts : Ts == typings env ts Ts"
 
-notation (xsymbols)
-  typing_rel  ("_ \<turnstile> _ : _" [50, 50, 50] 50)
-
 notation (latex)
   funs  (infixr "\<Rrightarrow>" 200) and
   typings_rel  ("_ \<tturnstile> _ : _" [50, 50, 50] 50)
-
-inductive typing
-  intros
-    Var [intro!]: "env x = T \<Longrightarrow> env \<turnstile> Var x : T"
-    Abs [intro!]: "env\<langle>0:T\<rangle> \<turnstile> t : U \<Longrightarrow> env \<turnstile> Abs t : (T \<Rightarrow> U)"
-    App [intro!]: "env \<turnstile> s : T \<Rightarrow> U \<Longrightarrow> env \<turnstile> t : T \<Longrightarrow> env \<turnstile> (s \<degree> t) : U"
-
-inductive_cases typing_elims [elim!]:
-  "e \<turnstile> Var i : T"
-  "e \<turnstile> t \<degree> u : T"
-  "e \<turnstile> Abs t : T"
 
 primrec
   "(e \<tturnstile> [] : Ts) = (Ts = [])"
@@ -100,16 +92,16 @@ lemma "e \<turnstile> Abs (Abs (Abs (Var 2 \<degree> Var 0 \<degree> (Var 1 \<de
 subsection {* Lists of types *}
 
 lemma lists_typings:
-    "e \<tturnstile> ts : Ts \<Longrightarrow> ts \<in> lists {t. \<exists>T. e \<turnstile> t : T}"
+    "e \<tturnstile> ts : Ts \<Longrightarrow> listsp (\<lambda>t. \<exists>T. e \<turnstile> t : T) ts"
   apply (induct ts arbitrary: Ts)
    apply (case_tac Ts)
      apply simp
-     apply (rule lists.Nil)
+     apply (rule listsp.Nil)
     apply simp
   apply (case_tac Ts)
    apply simp
   apply simp
-  apply (rule lists.Cons)
+  apply (rule listsp.Cons)
    apply blast
   apply blast
   done
@@ -172,7 +164,7 @@ lemma list_app_typeD:
   apply (erule impE)
    apply assumption
   apply (elim exE conjE)
-  apply (ind_cases "e \<turnstile> t \<degree> u : T")
+  apply (ind_cases2 "e \<turnstile> t \<degree> u : T" for t u T)
   apply (rule_tac x = "Ta # Ts" in exI)
   apply simp
   done
@@ -210,12 +202,12 @@ theorem var_app_type_eq:
   "e \<turnstile> Var i \<degree>\<degree> ts : T \<Longrightarrow> e \<turnstile> Var i \<degree>\<degree> ts : U \<Longrightarrow> T = U"
   apply (induct ts arbitrary: T U rule: rev_induct)
   apply simp
-  apply (ind_cases "e \<turnstile> Var i : T")
-  apply (ind_cases "e \<turnstile> Var i : T")
+  apply (ind_cases2 "e \<turnstile> Var i : T" for T)
+  apply (ind_cases2 "e \<turnstile> Var i : T" for T)
   apply simp
   apply simp
-  apply (ind_cases "e \<turnstile> t \<degree> u : T")
-  apply (ind_cases "e \<turnstile> t \<degree> u : T")
+  apply (ind_cases2 "e \<turnstile> t \<degree> u : T" for t u T)
+  apply (ind_cases2 "e \<turnstile> t \<degree> u : T" for t u T)
   apply atomize
   apply (erule_tac x="Ta \<Rightarrow> T" in allE)
   apply (erule_tac x="Tb \<Rightarrow> U" in allE)
@@ -238,7 +230,7 @@ lemma var_app_types: "e \<turnstile> Var i \<degree>\<degree> ts \<degree>\<degr
   apply (rule FalseE)
   apply simp
   apply (erule list_app_typeE)
-  apply (ind_cases "e \<turnstile> t \<degree> u : T")
+  apply (ind_cases2 "e \<turnstile> t \<degree> u : T" for t u T)
   apply (drule_tac T="Atom nat" and U="Ta \<Rightarrow> Tsa \<Rrightarrow> T" in var_app_type_eq)
   apply assumption
   apply simp
@@ -250,7 +242,7 @@ lemma var_app_types: "e \<turnstile> Var i \<degree>\<degree> ts \<degree>\<degr
   apply (rule types_snoc)
   apply assumption
   apply (erule list_app_typeE)
-  apply (ind_cases "e \<turnstile> t \<degree> u : T")
+  apply (ind_cases2 "e \<turnstile> t \<degree> u : T" for t u T)
   apply (drule_tac T="type1 \<Rightarrow> type2" and U="Ta \<Rightarrow> Tsa \<Rrightarrow> T" in var_app_type_eq)
   apply assumption
   apply simp
@@ -258,7 +250,7 @@ lemma var_app_types: "e \<turnstile> Var i \<degree>\<degree> ts \<degree>\<degr
   apply (rule typing.App)
   apply assumption
   apply (erule list_app_typeE)
-  apply (ind_cases "e \<turnstile> t \<degree> u : T")
+  apply (ind_cases2 "e \<turnstile> t \<degree> u : T" for t u T)
   apply (frule_tac T="type1 \<Rightarrow> type2" and U="Ta \<Rightarrow> Tsa \<Rrightarrow> T" in var_app_type_eq)
   apply assumption
   apply simp
@@ -266,7 +258,7 @@ lemma var_app_types: "e \<turnstile> Var i \<degree>\<degree> ts \<degree>\<degr
   apply (rule_tac x="type1 # Us" in exI)
   apply simp
   apply (erule list_app_typeE)
-  apply (ind_cases "e \<turnstile> t \<degree> u : T")
+  apply (ind_cases2 "e \<turnstile> t \<degree> u : T" for t u T)
   apply (frule_tac T="type1 \<Rightarrow> Us \<Rrightarrow> T" and U="Ta \<Rightarrow> Tsa \<Rrightarrow> T" in var_app_type_eq)
   apply assumption
   apply simp
@@ -281,13 +273,13 @@ lemma var_app_typesE: "e \<turnstile> Var i \<degree>\<degree> ts : T \<Longrigh
 lemma abs_typeE: "e \<turnstile> Abs t : T \<Longrightarrow> (\<And>U V. e\<langle>0:U\<rangle> \<turnstile> t : V \<Longrightarrow> P) \<Longrightarrow> P"
   apply (cases T)
   apply (rule FalseE)
-  apply (erule typing.elims)
+  apply (erule typing.cases)
   apply simp_all
   apply atomize
   apply (erule_tac x="type1" in allE)
   apply (erule_tac x="type2" in allE)
   apply (erule mp)
-  apply (erule typing.elims)
+  apply (erule typing.cases)
   apply simp_all
   done
 
@@ -335,14 +327,14 @@ lemma substs_lemma:
 
 subsection {* Subject reduction *}
 
-lemma subject_reduction: "e \<turnstile> t : T \<Longrightarrow> t -> t' \<Longrightarrow> e \<turnstile> t' : T"
+lemma subject_reduction: "e \<turnstile> t : T \<Longrightarrow> t \<rightarrow>\<^sub>\<beta> t' \<Longrightarrow> e \<turnstile> t' : T"
   apply (induct arbitrary: t' set: typing)
     apply blast
    apply blast
   apply atomize
-  apply (ind_cases "s \<degree> t -> t'")
+  apply (ind_cases2 "s \<degree> t \<rightarrow>\<^sub>\<beta> t'" for s t t')
     apply hypsubst
-    apply (ind_cases "env \<turnstile> Abs t : T \<Rightarrow> U")
+    apply (ind_cases2 "env \<turnstile> Abs t : T \<Rightarrow> U" for env t T U)
     apply (rule subst_lemma)
       apply assumption
      apply assumption
