src/HOL/MicroJava/J/TypeRel.thy
@@ -8,61 +8,45 @@ header {* \isaheader{Relations between Java Types} *}
 
 theory TypeRel imports Decl begin
 
-consts
-  subcls1 :: "'c prog => (cname \<times> cname) set"  -- "subclass"
-  widen   :: "'c prog => (ty    \<times> ty   ) set"  -- "widening"
-  cast    :: "'c prog => (ty    \<times> ty   ) set"  -- "casting"
-
-syntax (xsymbols)
-  subcls1 :: "'c prog => [cname, cname] => bool" ("_ \<turnstile> _ \<prec>C1 _" [71,71,71] 70)
-  subcls  :: "'c prog => [cname, cname] => bool" ("_ \<turnstile> _ \<preceq>C _"  [71,71,71] 70)
-  widen   :: "'c prog => [ty   , ty   ] => bool" ("_ \<turnstile> _ \<preceq> _"   [71,71,71] 70)
-  cast    :: "'c prog => [ty   , ty   ] => bool" ("_ \<turnstile> _ \<preceq>? _"  [71,71,71] 70)
-
-syntax
-  subcls1 :: "'c prog => [cname, cname] => bool" ("_ |- _ <=C1 _" [71,71,71] 70)
-  subcls  :: "'c prog => [cname, cname] => bool" ("_ |- _ <=C _"  [71,71,71] 70)
-  widen   :: "'c prog => [ty   , ty   ] => bool" ("_ |- _ <= _"   [71,71,71] 70)
-  cast    :: "'c prog => [ty   , ty   ] => bool" ("_ |- _ <=? _"  [71,71,71] 70)
-
-translations
-  "G\<turnstile>C \<prec>C1 D" == "(C,D) \<in> subcls1 G"
-  "G\<turnstile>C \<preceq>C  D" == "(C,D) \<in> (subcls1 G)^*"
-  "G\<turnstile>S \<preceq>   T" == "(S,T) \<in> widen   G"
-  "G\<turnstile>C \<preceq>?  D" == "(C,D) \<in> cast    G"
-
 -- "direct subclass, cf. 8.1.3"
-inductive "subcls1 G" intros
+inductive2
+  subcls1 :: "'c prog => [cname, cname] => bool" ("_ \<turnstile> _ \<prec>C1 _" [71,71,71] 70)
+  for G :: "'c prog"
+where
   subcls1I: "\<lbrakk>class G C = Some (D,rest); C \<noteq> Object\<rbrakk> \<Longrightarrow> G\<turnstile>C\<prec>C1D"
+
+abbreviation
+  subcls  :: "'c prog => [cname, cname] => bool" ("_ \<turnstile> _ \<preceq>C _"  [71,71,71] 70)
+  where "G\<turnstile>C \<preceq>C  D \<equiv> (subcls1 G)^** C D"
   
 lemma subcls1D: 
   "G\<turnstile>C\<prec>C1D \<Longrightarrow> C \<noteq> Object \<and> (\<exists>fs ms. class G C = Some (D,fs,ms))"
-apply (erule subcls1.elims)
+apply (erule subcls1.cases)
 apply auto
 done
 
 lemma subcls1_def2: 
-  "subcls1 G = 
+  "subcls1 G = member2
      (SIGMA C: {C. is_class G C} . {D. C\<noteq>Object \<and> fst (the (class G C))=D})"
-  by (auto simp add: is_class_def dest: subcls1D intro: subcls1I)
+  by (auto simp add: is_class_def expand_fun_eq dest: subcls1D intro: subcls1I)
 
-lemma finite_subcls1: "finite (subcls1 G)"
-apply(subst subcls1_def2)
+lemma finite_subcls1: "finite (Collect2 (subcls1 G))"
+apply(simp add: subcls1_def2)
 apply(rule finite_SigmaI [OF finite_is_class])
 apply(rule_tac B = "{fst (the (class G C))}" in finite_subset)
 apply  auto
 done
 
-lemma subcls_is_class: "(C,D) \<in> (subcls1 G)^+ ==> is_class G C"
+lemma subcls_is_class: "(subcls1 G)^++ C D ==> is_class G C"
 apply (unfold is_class_def)
-apply(erule trancl_trans_induct)
+apply(erule trancl_trans_induct')
 apply (auto dest!: subcls1D)
 done
 
 lemma subcls_is_class2 [rule_format (no_asm)]: 
   "G\<turnstile>C\<preceq>C D \<Longrightarrow> is_class G D \<longrightarrow> is_class G C"
 apply (unfold is_class_def)
-apply (erule rtrancl_induct)
+apply (erule rtrancl_induct')
 apply  (drule_tac [2] subcls1D)
 apply  auto
 done
@@ -70,18 +54,19 @@ done
 constdefs
   class_rec :: "'c prog \<Rightarrow> cname \<Rightarrow> 'a \<Rightarrow>
     (cname \<Rightarrow> fdecl list \<Rightarrow> 'c mdecl list \<Rightarrow> 'a \<Rightarrow> 'a) \<Rightarrow> 'a"
-  "class_rec G == wfrec ((subcls1 G)^-1)
+  "class_rec G == wfrec (Collect2 ((subcls1 G)^--1))
     (\<lambda>r C t f. case class G C of
          None \<Rightarrow> arbitrary
        | Some (D,fs,ms) \<Rightarrow> 
            f C fs ms (if C = Object then t else r D t f))"
 
-lemma class_rec_lemma: "wf ((subcls1 G)^-1) \<Longrightarrow> class G C = Some (D,fs,ms) \<Longrightarrow>
+lemma class_rec_lemma: "wfP ((subcls1 G)^--1) \<Longrightarrow> class G C = Some (D,fs,ms) \<Longrightarrow>
  class_rec G C t f = f C fs ms (if C=Object then t else class_rec G D t f)"
-  by (simp add: class_rec_def wfrec cut_apply [OF converseI [OF subcls1I]])
+  by (simp add: class_rec_def wfrec [to_pred]
+    cut_apply [OF Collect2I [where P="(subcls1 G)^--1"], OF conversepI, OF subcls1I])
 
 definition
-  "wf_class G = wf ((subcls1 G)^-1)"
+  "wf_class G = wfP ((subcls1 G)^--1)"
 
 lemma class_rec_func [code func]:
   "class_rec G C t f = (if wf_class G then
@@ -93,13 +78,14 @@ proof (cases "wf_class G")
   case False then show ?thesis by auto
 next
   case True
-  from `wf_class G` have wf: "wf ((subcls1 G)^-1)"
+  from `wf_class G` have wf: "wfP ((subcls1 G)^--1)"
     unfolding wf_class_def .
   show ?thesis
   proof (cases "class G C")
     case None
     with wf show ?thesis
-      by (simp add: class_rec_def wfrec cut_apply [OF converseI [OF subcls1I]])
+      by (simp add: class_rec_def wfrec [to_pred]
+        cut_apply [OF Collect2I [where P="(subcls1 G)^--1"], OF conversepI, OF subcls1I])
   next
     case (Some x) show ?thesis
     proof (cases x)
@@ -121,7 +107,7 @@ consts
 defs method_def: "method \<equiv> \<lambda>(G,C). class_rec G C empty (\<lambda>C fs ms ts.
                            ts ++ map_of (map (\<lambda>(s,m). (s,(C,m))) ms))"
 
-lemma method_rec_lemma: "[|class G C = Some (D,fs,ms); wf ((subcls1 G)^-1)|] ==>
+lemma method_rec_lemma: "[|class G C = Some (D,fs,ms); wfP ((subcls1 G)^--1)|] ==>
   method (G,C) = (if C = Object then empty else method (G,D)) ++  
   map_of (map (\<lambda>(s,m). (s,(C,m))) ms)"
 apply (unfold method_def)
@@ -135,7 +121,7 @@ done
 defs fields_def: "fields \<equiv> \<lambda>(G,C). class_rec G C []    (\<lambda>C fs ms ts.
                            map (\<lambda>(fn,ft). ((fn,C),ft)) fs @ ts)"
 
-lemma fields_rec_lemma: "[|class G C = Some (D,fs,ms); wf ((subcls1 G)^-1)|] ==>
+lemma fields_rec_lemma: "[|class G C = Some (D,fs,ms); wfP ((subcls1 G)^--1)|] ==>
  fields (G,C) = 
   map (\<lambda>(fn,ft). ((fn,C),ft)) fs @ (if C = Object then [] else fields (G,D))"
 apply (unfold fields_def)
@@ -156,56 +142,62 @@ done
 
 
 -- "widening, viz. method invocation conversion,cf. 5.3 i.e. sort of syntactic subtyping"
-inductive "widen G" intros 
+inductive2
+  widen   :: "'c prog => [ty   , ty   ] => bool" ("_ \<turnstile> _ \<preceq> _"   [71,71,71] 70)
+  for G :: "'c prog"
+where
   refl   [intro!, simp]:       "G\<turnstile>      T \<preceq> T"   -- "identity conv., cf. 5.1.1"
-  subcls         : "G\<turnstile>C\<preceq>C D ==> G\<turnstile>Class C \<preceq> Class D"
-  null   [intro!]:             "G\<turnstile>     NT \<preceq> RefT R"
+| subcls         : "G\<turnstile>C\<preceq>C D ==> G\<turnstile>Class C \<preceq> Class D"
+| null   [intro!]:             "G\<turnstile>     NT \<preceq> RefT R"
 
 -- "casting conversion, cf. 5.5 / 5.1.5"
 -- "left out casts on primitve types"
-inductive "cast G" intros
+inductive2
+  cast    :: "'c prog => [ty   , ty   ] => bool" ("_ \<turnstile> _ \<preceq>? _"  [71,71,71] 70)
+  for G :: "'c prog"
+where
   widen:  "G\<turnstile> C\<preceq> D ==> G\<turnstile>C \<preceq>? D"
-  subcls: "G\<turnstile> D\<preceq>C C ==> G\<turnstile>Class C \<preceq>? Class D"
+| subcls: "G\<turnstile> D\<preceq>C C ==> G\<turnstile>Class C \<preceq>? Class D"
 
 lemma widen_PrimT_RefT [iff]: "(G\<turnstile>PrimT pT\<preceq>RefT rT) = False"
 apply (rule iffI)
-apply (erule widen.elims)
+apply (erule widen.cases)
 apply auto
 done
 
 lemma widen_RefT: "G\<turnstile>RefT R\<preceq>T ==> \<exists>t. T=RefT t"
-apply (ind_cases "G\<turnstile>S\<preceq>T")
+apply (ind_cases2 "G\<turnstile>RefT R\<preceq>T")
 apply auto
 done
 
 lemma widen_RefT2: "G\<turnstile>S\<preceq>RefT R ==> \<exists>t. S=RefT t"
-apply (ind_cases "G\<turnstile>S\<preceq>T")
+apply (ind_cases2 "G\<turnstile>S\<preceq>RefT R")
 apply auto
 done
 
 lemma widen_Class: "G\<turnstile>Class C\<preceq>T ==> \<exists>D. T=Class D"
-apply (ind_cases "G\<turnstile>S\<preceq>T")
+apply (ind_cases2 "G\<turnstile>Class C\<preceq>T")
 apply auto
 done
 
 lemma widen_Class_NullT [iff]: "(G\<turnstile>Class C\<preceq>NT) = False"
 apply (rule iffI)
-apply (ind_cases "G\<turnstile>S\<preceq>T")
+apply (ind_cases2 "G\<turnstile>Class C\<preceq>NT")
 apply auto
 done
 
 lemma widen_Class_Class [iff]: "(G\<turnstile>Class C\<preceq> Class D) = (G\<turnstile>C\<preceq>C D)"
 apply (rule iffI)
-apply (ind_cases "G\<turnstile>S\<preceq>T")
+apply (ind_cases2 "G\<turnstile>Class C \<preceq> Class D")
 apply (auto elim: widen.subcls)
 done
 
 lemma widen_NT_Class [simp]: "G \<turnstile> T \<preceq> NT \<Longrightarrow> G \<turnstile> T \<preceq> Class D"
-by (ind_cases "G \<turnstile> T \<preceq> NT",  auto)
+by (ind_cases2 "G \<turnstile> T \<preceq> NT",  auto)
 
 lemma cast_PrimT_RefT [iff]: "(G\<turnstile>PrimT pT\<preceq>? RefT rT) = False"
 apply (rule iffI)
-apply (erule cast.elims)
+apply (erule cast.cases)
 apply auto
 done
 
@@ -223,7 +215,7 @@ proof -
   next
     case (subcls C D T)
     then obtain E where "T = Class E" by (blast dest: widen_Class)
-    with subcls show "G\<turnstile>Class C\<preceq>T" by (auto elim: rtrancl_trans)
+    with subcls show "G\<turnstile>Class C\<preceq>T" by auto
   next
     case (null R RT)
     then obtain rt where "RT = RefT rt" by (blast dest: widen_RefT)
