src/HOL/Lambda/ListBeta.thy
@@ -14,10 +14,10 @@ text {*
 
 abbreviation
   list_beta :: "dB list => dB list => bool"  (infixl "=>" 50) where
-  "rs => ss == (rs, ss) : step1 beta"
+  "rs => ss == step1 beta rs ss"
 
 lemma head_Var_reduction:
-  "Var n \<degree>\<degree> rs -> v \<Longrightarrow> \<exists>ss. rs => ss \<and> v = Var n \<degree>\<degree> ss"
+  "Var n \<degree>\<degree> rs \<rightarrow>\<^sub>\<beta> v \<Longrightarrow> \<exists>ss. rs => ss \<and> v = Var n \<degree>\<degree> ss"
   apply (induct u == "Var n \<degree>\<degree> rs" v arbitrary: rs set: beta)
      apply simp
     apply (rule_tac xs = rs in rev_exhaust)
@@ -29,14 +29,14 @@ lemma head_Var_reduction:
   done
 
 lemma apps_betasE [elim!]:
-  assumes major: "r \<degree>\<degree> rs -> s"
-    and cases: "!!r'. [| r -> r'; s = r' \<degree>\<degree> rs |] ==> R"
+  assumes major: "r \<degree>\<degree> rs \<rightarrow>\<^sub>\<beta> s"
+    and cases: "!!r'. [| r \<rightarrow>\<^sub>\<beta> r'; s = r' \<degree>\<degree> rs |] ==> R"
       "!!rs'. [| rs => rs'; s = r \<degree>\<degree> rs' |] ==> R"
       "!!t u us. [| r = Abs t; rs = u # us; s = t[u/0] \<degree>\<degree> us |] ==> R"
   shows R
 proof -
   from major have
-   "(\<exists>r'. r -> r' \<and> s = r' \<degree>\<degree> rs) \<or>
+   "(\<exists>r'. r \<rightarrow>\<^sub>\<beta> r' \<and> s = r' \<degree>\<degree> rs) \<or>
     (\<exists>rs'. rs => rs' \<and> s = r \<degree>\<degree> rs') \<or>
     (\<exists>t u us. r = Abs t \<and> rs = u # us \<and> s = t[u/0] \<degree>\<degree> us)"
     apply (induct u == "r \<degree>\<degree> rs" s arbitrary: r rs set: beta)
@@ -66,18 +66,18 @@ proof -
 qed
 
 lemma apps_preserves_beta [simp]:
-    "r -> s ==> r \<degree>\<degree> ss -> s \<degree>\<degree> ss"
+    "r \<rightarrow>\<^sub>\<beta> s ==> r \<degree>\<degree> ss \<rightarrow>\<^sub>\<beta> s \<degree>\<degree> ss"
   by (induct ss rule: rev_induct) auto
 
 lemma apps_preserves_beta2 [simp]:
     "r ->> s ==> r \<degree>\<degree> ss ->> s \<degree>\<degree> ss"
   apply (induct set: rtrancl)
    apply blast
-  apply (blast intro: apps_preserves_beta rtrancl_into_rtrancl)
+  apply (blast intro: apps_preserves_beta rtrancl.rtrancl_into_rtrancl)
   done
 
 lemma apps_preserves_betas [simp]:
-    "rs => ss \<Longrightarrow> r \<degree>\<degree> rs -> r \<degree>\<degree> ss"
+    "rs => ss \<Longrightarrow> r \<degree>\<degree> rs \<rightarrow>\<^sub>\<beta> r \<degree>\<degree> ss"
   apply (induct rs arbitrary: ss rule: rev_induct)
    apply simp
   apply simp
