src/HOL/Lambda/StrongNorm.thy
@@ -16,41 +16,38 @@ Felix Joachimski and Ralph Matthes \cite{Matthes-Joachimski-AML}.
 
 subsection {* Properties of @{text IT} *}
 
-lemma lift_IT [intro!]: "t \<in> IT \<Longrightarrow> lift t i \<in> IT"
+lemma lift_IT [intro!]: "IT t \<Longrightarrow> IT (lift t i)"
   apply (induct arbitrary: i set: IT)
     apply (simp (no_asm))
     apply (rule conjI)
      apply
       (rule impI,
        rule IT.Var,
-       erule lists.induct,
+       erule listsp.induct,
        simp (no_asm),
-       rule lists.Nil,
+       rule listsp.Nil,
        simp (no_asm),
-       erule IntE,
-       rule lists.Cons,
+       rule listsp.Cons,
        blast,
        assumption)+
      apply auto
    done
 
-lemma lifts_IT: "ts \<in> lists IT \<Longrightarrow> map (\<lambda>t. lift t 0) ts \<in> lists IT"
+lemma lifts_IT: "listsp IT ts \<Longrightarrow> listsp IT (map (\<lambda>t. lift t 0) ts)"
   by (induct ts) auto
 
-lemma subst_Var_IT: "r \<in> IT \<Longrightarrow> r[Var i/j] \<in> IT"
+lemma subst_Var_IT: "IT r \<Longrightarrow> IT (r[Var i/j])"
   apply (induct arbitrary: i j set: IT)
     txt {* Case @{term Var}: *}
     apply (simp (no_asm) add: subst_Var)
     apply
     ((rule conjI impI)+,
       rule IT.Var,
-      erule lists.induct,
+      erule listsp.induct,
       simp (no_asm),
-      rule lists.Nil,
+      rule listsp.Nil,
       simp (no_asm),
-      erule IntE,
-      erule CollectE,
-      rule lists.Cons,
+      rule listsp.Cons,
       fast,
       assumption)+
    txt {* Case @{term Lambda}: *}
@@ -65,21 +62,21 @@ lemma subst_Var_IT: "r \<in> IT \<Longrightarrow> r[Var i/j] \<in> IT"
    apply auto
   done
 
-lemma Var_IT: "Var n \<in> IT"
-  apply (subgoal_tac "Var n \<degree>\<degree> [] \<in> IT")
+lemma Var_IT: "IT (Var n)"
+  apply (subgoal_tac "IT (Var n \<degree>\<degree> [])")
    apply simp
   apply (rule IT.Var)
-  apply (rule lists.Nil)
+  apply (rule listsp.Nil)
   done
 
-lemma app_Var_IT: "t \<in> IT \<Longrightarrow> t \<degree> Var i \<in> IT"
+lemma app_Var_IT: "IT t \<Longrightarrow> IT (t \<degree> Var i)"
   apply (induct set: IT)
     apply (subst app_last)
     apply (rule IT.Var)
     apply simp
-    apply (rule lists.Cons)
+    apply (rule listsp.Cons)
      apply (rule Var_IT)
-    apply (rule lists.Nil)
+    apply (rule listsp.Nil)
    apply (rule IT.Beta [where ?ss = "[]", unfolded foldl_Nil [THEN eq_reflection]])
     apply (erule subst_Var_IT)
    apply (rule Var_IT)
@@ -94,26 +91,26 @@ lemma app_Var_IT: "t \<in> IT \<Longrightarrow> t \<degree> Var i \<in> IT"
 subsection {* Well-typed substitution preserves termination *}
 
 lemma subst_type_IT:
-  "\<And>t e T u i. t \<in> IT \<Longrightarrow> e\<langle>i:U\<rangle> \<turnstile> t : T \<Longrightarrow>
-    u \<in> IT \<Longrightarrow> e \<turnstile> u : U \<Longrightarrow> t[u/i] \<in> IT"
+  "\<And>t e T u i. IT t \<Longrightarrow> e\<langle>i:U\<rangle> \<turnstile> t : T \<Longrightarrow>
+    IT u \<Longrightarrow> e \<turnstile> u : U \<Longrightarrow> IT (t[u/i])"
   (is "PROP ?P U" is "\<And>t e T u i. _ \<Longrightarrow> PROP ?Q t e T u i U")
 proof (induct U)
   fix T t
   assume MI1: "\<And>T1 T2. T = T1 \<Rightarrow> T2 \<Longrightarrow> PROP ?P T1"
   assume MI2: "\<And>T1 T2. T = T1 \<Rightarrow> T2 \<Longrightarrow> PROP ?P T2"
-  assume "t \<in> IT"
+  assume "IT t"
   thus "\<And>e T' u i. PROP ?Q t e T' u i T"
   proof induct
     fix e T' u i
-    assume uIT: "u \<in> IT"
+    assume uIT: "IT u"
     assume uT: "e \<turnstile> u : T"
     {
-      case (Var n rs e_ T'_ u_ i_)
+      case (Var rs n e_ T'_ u_ i_)
       assume nT: "e\<langle>i:T\<rangle> \<turnstile> Var n \<degree>\<degree> rs : T'"
-      let ?ty = "{t. \<exists>T'. e\<langle>i:T\<rangle> \<turnstile> t : T'}"
+      let ?ty = "\<lambda>t. \<exists>T'. e\<langle>i:T\<rangle> \<turnstile> t : T'"
       let ?R = "\<lambda>t. \<forall>e T' u i.
-        e\<langle>i:T\<rangle> \<turnstile> t : T' \<longrightarrow> u \<in> IT \<longrightarrow> e \<turnstile> u : T \<longrightarrow> t[u/i] \<in> IT"
-      show "(Var n \<degree>\<degree> rs)[u/i] \<in> IT"
+        e\<langle>i:T\<rangle> \<turnstile> t : T' \<longrightarrow> IT u \<longrightarrow> e \<turnstile> u : T \<longrightarrow> IT (t[u/i])"
+      show "IT ((Var n \<degree>\<degree> rs)[u/i])"
       proof (cases "n = i")
         case True
         show ?thesis
@@ -134,13 +131,13 @@ proof (induct U)
           from varT True have T: "T = T'' \<Rightarrow> Ts \<Rrightarrow> T'"
             by cases auto
           with uT have uT': "e \<turnstile> u : T'' \<Rightarrow> Ts \<Rrightarrow> T'" by simp
-          from T have "(Var 0 \<degree>\<degree> map (\<lambda>t. lift t 0)
-            (map (\<lambda>t. t[u/i]) as))[(u \<degree> a[u/i])/0] \<in> IT"
+          from T have "IT ((Var 0 \<degree>\<degree> map (\<lambda>t. lift t 0)
+            (map (\<lambda>t. t[u/i]) as))[(u \<degree> a[u/i])/0])"
           proof (rule MI2)
-            from T have "(lift u 0 \<degree> Var 0)[a[u/i]/0] \<in> IT"
+            from T have "IT ((lift u 0 \<degree> Var 0)[a[u/i]/0])"
             proof (rule MI1)
-              have "lift u 0 \<in> IT" by (rule lift_IT)
-              thus "lift u 0 \<degree> Var 0 \<in> IT" by (rule app_Var_IT)
+              have "IT (lift u 0)" by (rule lift_IT)
+              thus "IT (lift u 0 \<degree> Var 0)" by (rule app_Var_IT)
               show "e\<langle>0:T''\<rangle> \<turnstile> lift u 0 \<degree> Var 0 : Ts \<Rrightarrow> T'"
               proof (rule typing.App)
                 show "e\<langle>0:T''\<rangle> \<turnstile> lift u 0 : T'' \<Rightarrow> Ts \<Rrightarrow> T'"
@@ -149,19 +146,19 @@ proof (induct U)
                   by (rule typing.Var) simp
               qed
               from Var have "?R a" by cases (simp_all add: Cons)
-              with argT uIT uT show "a[u/i] \<in> IT" by simp
+              with argT uIT uT show "IT (a[u/i])" by simp
               from argT uT show "e \<turnstile> a[u/i] : T''"
                 by (rule subst_lemma) simp
             qed
-            thus "u \<degree> a[u/i] \<in> IT" by simp
-            from Var have "as \<in> lists {t. ?R t}"
+            thus "IT (u \<degree> a[u/i])" by simp
+            from Var have "listsp ?R as"
               by cases (simp_all add: Cons)
-            moreover from argsT have "as \<in> lists ?ty"
+            moreover from argsT have "listsp ?ty as"
               by (rule lists_typings)
-            ultimately have "as \<in> lists ({t. ?R t} \<inter> ?ty)"
-              by (rule lists_IntI)
-            hence "map (\<lambda>t. lift t 0) (map (\<lambda>t. t[u/i]) as) \<in> lists IT"
-              (is "(?ls as) \<in> _")
+            ultimately have "listsp (\<lambda>t. ?R t \<and> ?ty t) as"
+              by simp
+            hence "listsp IT (map (\<lambda>t. lift t 0) (map (\<lambda>t. t[u/i]) as))"
+              (is "listsp IT (?ls as)")
             proof induct
               case Nil
               show ?case by fastsimp
@@ -169,13 +166,13 @@ proof (induct U)
               case (Cons b bs)
               hence I: "?R b" by simp
               from Cons obtain U where "e\<langle>i:T\<rangle> \<turnstile> b : U" by fast
-              with uT uIT I have "b[u/i] \<in> IT" by simp
-              hence "lift (b[u/i]) 0 \<in> IT" by (rule lift_IT)
-              hence "lift (b[u/i]) 0 # ?ls bs \<in> lists IT"
-                by (rule lists.Cons) (rule Cons)
+              with uT uIT I have "IT (b[u/i])" by simp
+              hence "IT (lift (b[u/i]) 0)" by (rule lift_IT)
+              hence "listsp IT (lift (b[u/i]) 0 # ?ls bs)"
+                by (rule listsp.Cons) (rule Cons)
               thus ?case by simp
             qed
-            thus "Var 0 \<degree>\<degree> ?ls as \<in> IT" by (rule IT.Var)
+            thus "IT (Var 0 \<degree>\<degree> ?ls as)" by (rule IT.Var)
             have "e\<langle>0:Ts \<Rrightarrow> T'\<rangle> \<turnstile> Var 0 : Ts \<Rrightarrow> T'"
               by (rule typing.Var) simp
             moreover from uT argsT have "e \<tturnstile> map (\<lambda>t. t[u/i]) as : Ts"
@@ -194,13 +191,13 @@ proof (induct U)
         qed
       next
         case False
-        from Var have "rs \<in> lists {t. ?R t}" by simp
+        from Var have "listsp ?R rs" by simp
         moreover from nT obtain Ts where "e\<langle>i:T\<rangle> \<tturnstile> rs : Ts"
           by (rule list_app_typeE)
-        hence "rs \<in> lists ?ty" by (rule lists_typings)
-        ultimately have "rs \<in> lists ({t. ?R t} \<inter> ?ty)"
-          by (rule lists_IntI)
-        hence "map (\<lambda>x. x[u/i]) rs \<in> lists IT"
+        hence "listsp ?ty rs" by (rule lists_typings)
+        ultimately have "listsp (\<lambda>t. ?R t \<and> ?ty t) rs"
+          by simp
+        hence "listsp IT (map (\<lambda>x. x[u/i]) rs)"
         proof induct
           case Nil
           show ?case by fastsimp
@@ -208,9 +205,9 @@ proof (induct U)
           case (Cons a as)
           hence I: "?R a" by simp
           from Cons obtain U where "e\<langle>i:T\<rangle> \<turnstile> a : U" by fast
-          with uT uIT I have "a[u/i] \<in> IT" by simp
-          hence "(a[u/i] # map (\<lambda>t. t[u/i]) as) \<in> lists IT"
-            by (rule lists.Cons) (rule Cons)
+          with uT uIT I have "IT (a[u/i])" by simp
+          hence "listsp IT (a[u/i] # map (\<lambda>t. t[u/i]) as)"
+            by (rule listsp.Cons) (rule Cons)
           thus ?case by simp
         qed
         with False show ?thesis by (auto simp add: subst_Var)
@@ -219,29 +216,29 @@ proof (induct U)
       case (Lambda r e_ T'_ u_ i_)
       assume "e\<langle>i:T\<rangle> \<turnstile> Abs r : T'"
         and "\<And>e T' u i. PROP ?Q r e T' u i T"
-      with uIT uT show "Abs r[u/i] \<in> IT"
+      with uIT uT show "IT (Abs r[u/i])"
         by fastsimp
     next
       case (Beta r a as e_ T'_ u_ i_)
       assume T: "e\<langle>i:T\<rangle> \<turnstile> Abs r \<degree> a \<degree>\<degree> as : T'"
       assume SI1: "\<And>e T' u i. PROP ?Q (r[a/0] \<degree>\<degree> as) e T' u i T"
       assume SI2: "\<And>e T' u i. PROP ?Q a e T' u i T"
-      have "Abs (r[lift u 0/Suc i]) \<degree> a[u/i] \<degree>\<degree> map (\<lambda>t. t[u/i]) as \<in> IT"
+      have "IT (Abs (r[lift u 0/Suc i]) \<degree> a[u/i] \<degree>\<degree> map (\<lambda>t. t[u/i]) as)"
       proof (rule IT.Beta)
         have "Abs r \<degree> a \<degree>\<degree> as \<rightarrow>\<^sub>\<beta> r[a/0] \<degree>\<degree> as"
           by (rule apps_preserves_beta) (rule beta.beta)
         with T have "e\<langle>i:T\<rangle> \<turnstile> r[a/0] \<degree>\<degree> as : T'"
           by (rule subject_reduction)
-        hence "(r[a/0] \<degree>\<degree> as)[u/i] \<in> IT"
+        hence "IT ((r[a/0] \<degree>\<degree> as)[u/i])"
           by (rule SI1)
-        thus "r[lift u 0/Suc i][a[u/i]/0] \<degree>\<degree> map (\<lambda>t. t[u/i]) as \<in> IT"
+        thus "IT (r[lift u 0/Suc i][a[u/i]/0] \<degree>\<degree> map (\<lambda>t. t[u/i]) as)"
           by (simp del: subst_map add: subst_subst subst_map [symmetric])
         from T obtain U where "e\<langle>i:T\<rangle> \<turnstile> Abs r \<degree> a : U"
           by (rule list_app_typeE) fast
         then obtain T'' where "e\<langle>i:T\<rangle> \<turnstile> a : T''" by cases simp_all
-        thus "a[u/i] \<in> IT" by (rule SI2)
+        thus "IT (a[u/i])" by (rule SI2)
       qed
-      thus "(Abs r \<degree> a \<degree>\<degree> as)[u/i] \<in> IT" by simp
+      thus "IT ((Abs r \<degree> a \<degree>\<degree> as)[u/i])" by simp
     }
   qed
 qed
@@ -251,7 +248,7 @@ subsection {* Well-typed terms are strongly normalizing *}
 
 lemma type_implies_IT:
   assumes "e \<turnstile> t : T"
-  shows "t \<in> IT"
+  shows "IT t"
   using prems
 proof induct
   case Var
@@ -260,14 +257,14 @@ next
   case Abs
   show ?case by (rule IT.Lambda)
 next
-  case (App T U e s t)
-  have "(Var 0 \<degree> lift t 0)[s/0] \<in> IT"
+  case (App e s T U t)
+  have "IT ((Var 0 \<degree> lift t 0)[s/0])"
   proof (rule subst_type_IT)
-    have "lift t 0 \<in> IT" by (rule lift_IT)
-    hence "[lift t 0] \<in> lists IT" by (rule lists.Cons) (rule lists.Nil)
-    hence "Var 0 \<degree>\<degree> [lift t 0] \<in> IT" by (rule IT.Var)
+    have "IT (lift t 0)" by (rule lift_IT)
+    hence "listsp IT [lift t 0]" by (rule listsp.Cons) (rule listsp.Nil)
+    hence "IT (Var 0 \<degree>\<degree> [lift t 0])" by (rule IT.Var)
     also have "Var 0 \<degree>\<degree> [lift t 0] = Var 0 \<degree> lift t 0" by simp
-    finally show "\<dots> \<in> IT" .
+    finally show "IT \<dots>" .
     have "e\<langle>0:T \<Rightarrow> U\<rangle> \<turnstile> Var 0 : T \<Rightarrow> U"
       by (rule typing.Var) simp
     moreover have "e\<langle>0:T \<Rightarrow> U\<rangle> \<turnstile> lift t 0 : T"
@@ -278,10 +275,10 @@ next
   thus ?case by simp
 qed
 
-theorem type_implies_termi: "e \<turnstile> t : T \<Longrightarrow> t \<in> termi beta"
+theorem type_implies_termi: "e \<turnstile> t : T \<Longrightarrow> termi beta t"
 proof -
   assume "e \<turnstile> t : T"
-  hence "t \<in> IT" by (rule type_implies_IT)
+  hence "IT t" by (rule type_implies_IT)
   thus ?thesis by (rule IT_implies_termi)
 qed
 
